update dict with tree

src/dict.v
@@ -14,25 +14,36 @@ Section Dict.
 
   Variable hash: A -> positive.
 
-  Definition t := tree (list (A * B)).
+  Inductive bucket_e : Set :=
+    | C : positive -> A -> B  -> bucket_e.
+  Definition t := tree (list (bucket_e)).
 
   Definition empty : t := empty.
+
+  Fixpoint find_iter h_k k l: option B :=
+    match l with
+    | nil     => None
+    | C h k' v :: tl => 
+        if h_k =? h
+        then ( if eq k k' 
+               then Some v
+               else find_iter h_k k tl) 
+        else find_iter h_k k tl
+    end.
 
   Definition find (k: A) (d: t): option B :=
     match get (hash k) d with
     | None   => None
-    | Some l => find_snd A B (fun '(k', _) => eq k k') l
+    | Some l => find_iter (hash k) k l
     end.
 
   Definition add (k: A) (e: B) (d: t): t := 
     let h_k := hash k in
     match get h_k d with
-    | None   => set h_k [(k, e)] d
-    | Some l => set h_k ((k, e)::l) d
+    | None   => set h_k [ C h_k k e ] d
+    | Some l => set h_k ( C h_k k e :: l ) d
     end.
   
-  Search reflect.
-
   Lemma eq_true:
     forall (k1 k2 : A), k1 = k2 -> eq k1 k2 = true.
   Proof.
@@ -68,16 +79,21 @@ Section Dict.
     intros k x d. unfold find, add.
     case (get (hash k) d).
     - intro l. rewrite gss. simpl. 
-      case (eq_spec k k). now intro. contradiction.
+      case (eq_spec k k). intros Hk.
+      assert (H: hash k =? hash k = true) by now rewrite Pos.eqb_eq.
+      now rewrite H.
+      intros Hk. contradiction.
     - rewrite gss. simpl.
-      case (eq_spec k k). now intro. contradiction.
+      case (eq_spec k k); intros Hk.
+      assert (H: hash k =? hash k = true) by now rewrite Pos.eqb_eq.
+      now rewrite H. contradiction.
   Qed.
 
   Lemma hash_equal:
-    forall (k1 k2: A) (x: B) (d: t) (l: list (A * B)),
+    forall (k1 k2: A) (x: B) (d: t) l,
       hash k1 = hash k2 -> 
       get (hash k1) d = Some l -> 
-      get (hash k1) (add k2 x d) = Some ((k2, x) :: l).
+      get (hash k1) (add k2 x d) = Some (C (hash k2) k2 x :: l).
   Proof.
     intros k1 k2 x d l H Hget.
     unfold add. rewrite <- H. rewrite Hget.
@@ -85,7 +101,7 @@ Section Dict.
   Qed.
 
   Lemma hash_diff:
-    forall (k1 k2: A) (x: B) (d: t) (l: option (list (A *B))),
+    forall (k1 k2: A) (x: B) (d: t) l,
       hash k1 <> hash k2 -> 
       get (hash k1) d = l -> 
       get (hash k1) (add k2 x d) = l.
@@ -105,12 +121,44 @@ Section Dict.
     - intros Heq. 
       destruct (get (hash k1) d) eqn:Hget.
       rewrite hash_equal with (1 := Heq) (2 := Hget). 
-      simpl. case (eq_spec k1 k2). easy. now intros _.
-      rewrite Heq. unfold add.
-      rewrite <- Heq, Hget. rewrite gss. simpl.
-      case (eq_spec k1 k2). easy. now intros _.
+      simpl. rewrite <- Pos.eqb_eq in Heq. rewrite Heq.
+      assert (H0: eq k1 k2 = false) by now rewrite eq_false.
+      now rewrite H0.
+      unfold add. rewrite <- Heq, Hget. rewrite gss. simpl.
+      assert (H0: hash k1 =? hash k1 = true) by now rewrite Pos.eqb_eq.
+      rewrite H0. assert (H1: eq k1 k2 = false) by now rewrite eq_false.
+      now rewrite H1.
     - intro Hdiff. case (get (hash k1) d) eqn:Hget;
       now rewrite hash_diff with (1 := Hdiff) (2 := Hget).
   Qed.
 End Dict.
+
+Module Type Hash_type.
+  Variable A: Set.
+  Variable eq: A -> A -> bool.
+  Variable eq_spec: forall x y : A, reflect (x = y) (eq x y).
+  Variable hash: A -> positive.
+End Hash_type.
+
+Module HashTable (T: Hash_type).
+  Definition t := @t T.A.
+  Definition create (B: Set) : t B :=
+    empty T.A B.
+
+  Definition add {B: Set} (h: t B) (key: T.A) (v: B) :=
+    add T.A B T.hash key v h.
+
+  Definition find {B: Set} (h: t B) (key: T.A): option B :=
+    find T.A T.eq B T.hash key h.
+End HashTable.
+
+Check Pos.eqb_spec.
+
+Module Int <: Hash_type.
+  Definition A := positive.
+  Definition eq x y:= Pos.eqb x y.
+  Definition eq_spec := Pos.eqb_spec.
+  Definition hash i: A := i.
+End Int.
+
 
