src/tree.v
@@ -1,9 +1,0 @@
-Module Type TREE.
-  Parameter elt: Type.
-  Parameter elt_eq: forall (a b :elt), {a = b} + {a <> b}.
-  Parameter t: Type -> Type.
-  Parameter empty: forall (A: Type), t A.
-  Parameter get: forall (A: Type), elt -> t A -> option A.
-  Parameter set: forall (A: Type), elt -> A -> t A -> t A.
-End TREE.
-
